

Discrete Mathematics

from 93APM3 Applied Mathematics 3

AY25/26 Sem 2

This set of notes is based on the lectures as delivered in AY25/26 by Dr Li Zhongqiang,
with reference to *Discrete Mathematics and Its Applications* (Rosen, 2019).

Contents

1	Sets	3
1.1	Basic Set Notation	3
1.2	Algebra of Sets	3
2	Logic and Proofs	3
2.1	Propositional Logic	3
2.2	Propositional Equivalences	4
2.3	Predicates and Quantifiers	5
2.4	Proofs, Methods for Proofs	5
2.4.1	Terminology	5
2.5	Methods of Proof	6
2.5.1	Direct Proof	6
2.5.2	Indirect Proof	6
2.5.3	Proof by Contradiction	6
2.5.4	Proof by Induction	7

Sets

1.1 Basic Set Notation

notation	definition
\in	is an element of.
\notin	is not an element of.
$A = \{x_1, x_2, \dots\}$	list of elements of A .
$A = \{x : x \in \mathbb{R}\}$	rule by which elements of A are determined.
$A \subset B$	A is a subset of B .
$A \subseteq B$	A is a proper subset of B . $A \subset B$, $A \neq B$.
U	Universal set of all elements of interest.
\emptyset	The empty set.
\overline{A} or A^c	$\overline{A} = \{x, x \in U, x \notin A\}$.
$A \cup B$	set of all the elements of A and B .
$A \cap B$	set of the common elements of A and B .

A disjointed set is the set of A and B such that

$$A \cap B = \emptyset.$$

1.2 Algebra of Sets

Commutative law: $A \cup B \equiv B \cup A$, $A \cap B \equiv B \cap A$

Idempotent law: $A \cup A = A$, $A \cap A = A$

Identity law: $A \cup \emptyset = A$, $A \cap U = A$

Complementary law: $A \cup \overline{A} = U$, $A \cap \overline{A} = \emptyset$

Associative law: $A \cup (B \cup C) = (A \cup B) \cup C$

Distributive law: $A \cup (B \cap C) = (A \cup B) \cap (A \cup C)$

De Morgan laws: $\overline{A \cup B} = \overline{A} \cap \overline{B}$, $\overline{A \cap B} = \overline{A} \cup \overline{B}$

Logic and Proofs

2.1 Propositional Logic

Definition 2.1.1. The proposition p is a statement which declares a fact, and which is immediately discernible as either true or false.

Remarks. Compound propositions can be created through the application of logical operators on a proposition.

Definition 2.1.2. The *negation* of p , \tilde{p} is the statement "it is not the case that p ".

Remarks. \tilde{p} can also be written \overline{p} or $\neg p$

Definition 2.1.3. The *conjunction* of p and q , $p \wedge q$ is the statement " p and q ".

Definition 2.1.4. The *disjunction* of p and q , $p \vee q$ is the statement " p or q ".

Definition 2.1.5. The *exclusive or* of p and q , $p \oplus q$ is the statement which is true when, and only when, either p or q is true, but not both.

Definition 2.1.6. The *implication* $p \Rightarrow q$ is the statement " p implies q ".

Remarks. The statement $p \rightarrow r$ is the *hypothesis*. q is the conclusion. Remember that just because q is true, this does **not** mean that p is true. This relation is not reversible.

Definition 2.1.7. The *converse* of the statement $p \Rightarrow q$ is the statement $q \Rightarrow p$.

Definition 2.1.8. The *contrapositive* of $p \Rightarrow q$ is $\neg q \Rightarrow \neg p$.

Definition 2.1.9. The *bi-conditional* statement $p \iff q$ is the proposition " p if and only if q ".

Remarks. The bi-conditional is the compound proposition of $p \Rightarrow q$ and $q \Rightarrow p$. A true result is returned only when both p and q have the same truth table values, and is false otherwise. It has the same truth table values as $(p \Rightarrow q) \wedge (q \Rightarrow p)$.

2.2 Propositional Equivalences

Definition 2.2.1. The *contradiction* is a statement which is always false.

Remarks. For example, the statement $s \equiv p \wedge \tilde{p}$ is always false. It is thus a contradiction.

Definition 2.2.2. The *tautology* is a statement which is always true.

Remarks. For example, the statement $t \equiv p \vee \tilde{p}$ is always true. It is thus a tautology.

Definition 2.2.3. The compound propositions p and q are called *logically equivalent* if $p \iff q$ is a tautology (always true). This is also denoted with $p \equiv q$.

The table below illustrates a number of such logical equivalences.

name	equivalence
identity laws	$p \wedge t \equiv p$ $p \vee s \equiv p$
domination laws	$p \vee t \equiv t$ $p \wedge s \equiv s$
idempotent laws	$p \vee p \equiv p$ $p \wedge p \equiv p$
double negation law	$\neg(\tilde{p}) \equiv p$
associative law	$(p \vee q) \vee r \equiv p \vee (q \vee r)$ $(p \wedge q) \wedge r \equiv p \wedge (q \wedge r)$
distributive law	$p \vee (p \wedge r) \equiv (p \vee q) \wedge (p \vee r)$ $p \wedge (p \vee r) \equiv (p \wedge q) \vee (p \wedge r)$
De Morgan's laws	$\overline{(p \vee q)} \equiv \tilde{p} \wedge \tilde{q}$ $\overline{(p \wedge q)} \equiv \tilde{p} \vee \tilde{q}$
absorption laws	$p \wedge (p \vee q) \equiv p$ $p \vee (p \wedge q) \equiv p$
complementary(negation) law	$p \vee \tilde{p} \equiv t$ $p \wedge \tilde{p} \equiv s$

2.3 Predicates and Quantifiers

Definition 2.3.1. The *Propositional Function* $P(x)$ refers to a statement which becomes a proposition when a value is assigned to its *variable(s)* a, b, \dots, z . The *predicate* is the condition to be fulfilled.

Exercise. Take $x > 3$. This propositional function only becomes a proposition when we give x a value, such that we can determine the function's truth table.

2.4 Proofs, Methods for Proofs

2.4.1 Terminology

word	definition
theorem	a statement that can be shown to be true (also: facts, results).
proposition	a less important theorem.
proof	demonstration that a theorem is true.
axioms	statements we assume to be true (also: postulates).
lemma	a less important theorem useful in the proof of other results.
corollary	theorem that can be directly established from a theorem that has been proved.
conjecture	a statement which is proposed to be a true statement.

2.5 Methods of Proof

2.5.1 Direct Proof

The *direct proof* of the proposition $p \rightarrow q$ is one which begins with the assumption that p is true, before the usage of a series of axioms, definitions, and proved theories, to show that q is also true. Direct proofs are the most straightforward of the proofs.

Definition 2.5.1. An integer n is even if there exists an integer k such that $n = 2k$, and n is odd if there exists an integer k such that $n = 2k + 1$. Two integers are said to have the same *parity* when both are even or both are odd; they have the opposite parity when one is even and the other is odd.

Exercise. If n is odd, prove that n^2 is odd.

$$n = 2k + 1, k \in \mathbb{Z} \quad (1)$$

$$n^2 = (2k + 1)^2 \quad (2)$$

$$= 2(2k^2 + 2k) + 1 \quad (3)$$

therefore, by definition, n^2 is odd.

2.5.2 Indirect Proof

An *indirect proof* is one which does not start with the premise and end with the conclusion.

Proof by contraposition: We utilise the fact that the implication $p \rightarrow q$ is equivalent to its contrapositive $\tilde{p} \rightarrow \tilde{q}$. Taking \tilde{p} as the premise, we use axioms, definitions and proven theorems to show that \tilde{q} must follow. This indirectly proves that $p \implies q$.

Vacuous proof: Given that p is false, then it follows that $p \rightarrow q$ must be true. Therefore, if we can prove that p is false, we can then establish the *vacuous proof*.

Trivial proof: Given that q is true, then it follows that $p \implies q$ is also true. Such a proof is known as the *trivial proof*.

2.5.3 Proof by Contradiction

We prove the statement p is true when we prove that $\tilde{p} \rightarrow (r \wedge \tilde{r})$, or $\tilde{p} \rightarrow \text{false}$.

Exercise. Prove $\sqrt{2}$ is irrational.

If $\sqrt{2}$ is rational, then

$$\sqrt{2} = \frac{m}{n} \quad (4)$$

where m, n have no common factors. Squaring both sides, we get

$$2n^2 = m^2, \quad (5)$$

which implies

$$m = 2k.$$

Thus,

$$m^2 = 4k^2 \tag{6}$$

However, from 5,

$$n^2 = \frac{1}{2}m^2 = 2k^2 \rightarrow n^2 \text{ is odd.}$$

Since both m and n are odd, they therefore have a common factor of 2. We have proven that $\sqrt{2}$ is irrational by contradiction.

2.5.4 Proof by Induction

Suppose we have the statements $p_1, p_2, p_3, \dots, p_n, n \in \mathbb{N}$. If we prove that p_1 is true (the basis for induction), then we assume p_k is true. This is the induction hypothesis. We then show that p_{k+1} is true, which proves that p_n is true by induction.